Generic EnvMap (#658)
* Integrate removal of parameters in the erasure, and refactor optimization proofs

* Use a faster (but harder to reason about definition of strip) so that erasure computes fast in Coq and in OCaml

* Fixup _PluginProject.in

* Make Environment maps generic in the declarations to be reused in template and erasure

* Move EnvMap to template, make it polymorphic and use it in the template -> PCUIC translation too

* Adapt Template -> PCUIC correctness to efficient global env implemetation

* Use lookup tables consistently in erasure

* Fix erasure to stop rebuilding the lookup environment at each declaration. We're down to 1sec for self-erasure

* Also use EnvMaps in RemoveParams, optimizing it some more

* Fix old dependencies on PCUICEnvMap

* #657 + #658 (#660)

* WIP: erase and erasure relation agree on firstorder inductives

* better now

* down to one admit and one todo

* Proved progress for wcbv reduction

* add vscode file

* prove WN without cofix

* consolidate into different files

* start eta expansion pass

* erasure keeps eta expansion

* eta expand only non-erased parts

* prove eta expansion for template correct

* done eta expand

* factor out things into EExtends.v

* fix compilation

* Parameter stripping integration (#656)

* Integrate removal of parameters in the erasure, and refactor optimization proofs

* Use a faster (but harder to reason about definition of strip) so that erasure computes fast in Coq and in OCaml

* Fixup _PluginProject.in

* fix compilation

* remove plugin

* fix compilation on coq-8.14 branch

* fix PluginProject and mlpack

* fix compilation

Co-authored-by: Matthieu Sozeau <matthieu.sozeau@inria.fr>

Co-authored-by: Yannick Forster <yannick.forster@inria.fr>

erasure/theories/Erasure.v
@@ -16,13 +16,17 @@ From MetaCoq.Erasure Require ErasureFunction EOptimizePropDiscr ERemoveParams EW
      indices_matter := false;
      lets_in_constructor_types := true |}.
 
+(* Used to show timings of the ML execution *)
+ 
+Definition time : forall {A}, string -> (unit -> A) -> unit -> A :=
+  fun A s f x => f x.
+
+Extract Constant time => "(fun c f x -> let s = Tm_util.list_to_string c in Tm_util.time (Pp.str s) f x)".
+
 (* This is the total erasure function +
   let-expansion of constructor arguments and case branches +
   shrinking of the global environment dependencies +
   the optimization that removes all pattern-matches on propositions. *)
-
-Definition eprogram := 
-  (EAst.global_context * EAst.term).
 
 Import EOptimizePropDiscr.
 
@@ -41,13 +45,16 @@ Module Transform.
         ∥ eval' p' v' × obseq p p' v v' ∥.
 
     Record t := 
-    { pre : program -> Prop; 
+    { name : string; 
+      pre : program -> Prop; 
       transform : forall p : program, pre p -> program';
       post : program' -> Prop;
       correctness : forall input (p : pre input), post (transform input p);
       obseq : program -> program' -> value -> value' -> Prop;
-      preservation : preserves_eval pre transform obseq; 
-      }.
+      preservation : preserves_eval pre transform obseq; }.
+
+    Definition run (x : t) (p : program) (pr : pre x p) : program' := 
+      time x.(name) (fun _ => x.(transform) p pr) tt.
 
   End Opt.
   Arguments t : clear implicits.
@@ -63,7 +70,8 @@ Module Transform.
     Program Definition compose (o : t program program' value value' eval eval') (o' : t program' program'' value' value'' eval' eval'') 
       (hpp : (forall p, o.(post) p -> o'.(pre) p)) : t program program'' value value'' eval eval'' :=
       {| 
-        transform p hp := o'.(transform) (o.(transform) p hp) (hpp _ (o.(correctness) _ hp));
+        name := o.(name) ^ " -> " ^ o'.(name);
+        transform p hp := run o' (run o p hp) (hpp _ (o.(correctness) _ hp));
         pre := o.(pre);
         post := o'.(post);
         obseq g g' v v' := exists g'' v'', o.(obseq) g g'' v v'' × o'.(obseq) g'' g' v'' v'
@@ -88,19 +96,27 @@ Module Transform.
 End Transform.
 Import ETyping.
 
-Definition self_optimization program value eval eval' := Transform.t program program value value eval eval'.
+Definition self_transform program value eval eval' := Transform.t program program value value eval eval'.
+
+Definition eprogram := 
+  (EAst.global_context * EAst.term).
+
+Import EEtaExpanded.GlobalContextMap (make, global_decls).
 
 Definition eval_eprogram (wfl : EWcbvEval.WcbvFlags) (p : eprogram) (t : EAst.term) := 
   EWcbvEval.eval (wfl:=wfl) p.1 p.2 t.
 
 Import Transform.
 Obligation Tactic := idtac.
-Program Definition optimize_prop_discr_optimization : self_optimization eprogram EAst.term (eval_eprogram EWcbvEval.default_wcbv_flags) (eval_eprogram EWcbvEval.opt_wcbv_flags) := 
-  {| transform p _ := (EOptimizePropDiscr.optimize_env p.1, EOptimizePropDiscr.optimize p.1 p.2);
+Program Definition optimize_prop_discr_optimization : self_transform eprogram EAst.term (eval_eprogram EWcbvEval.default_wcbv_flags) (eval_eprogram EWcbvEval.opt_wcbv_flags) := 
+  {| name := "optimize_prop_discr"; 
+    transform p _ := 
+      (EOptimizePropDiscr.optimize_env p.1, EOptimizePropDiscr.optimize p.1 p.2);
     pre p := (closed_env p.1 /\ ELiftSubst.closedn 0 p.2);
     post p := (closed_env p.1 /\ ELiftSubst.closedn 0 p.2);
     obseq g g' v v' := v' = EOptimizePropDiscr.optimize g.1 v
     |}.
+
 Next Obligation.
   intros [Σ t] [cle clt].
   cbn in *. split.
@@ -116,10 +132,56 @@ Next Obligation.
   eapply EOptimizePropDiscr.optimize_correct in ev; eauto.
 Qed.
 
-Program Definition remove_params_optimization (fl : EWcbvEval.WcbvFlags) : self_optimization eprogram EAst.term (eval_eprogram fl) (eval_eprogram fl) :=
-  {|
+Lemma wf_glob_fresh Σ : wf_glob Σ -> EnvMap.EnvMap.fresh_globals Σ.
+Proof.
+  induction Σ. constructor; auto.
+  intros wf; depelim wf. constructor; auto.
+Qed.
+
+Definition eprogram_env := 
+  (EEtaExpanded.GlobalContextMap.t * EAst.term).
+
+Definition eval_eprogram_env (wfl : EWcbvEval.WcbvFlags) (p : eprogram_env) (t : EAst.term) := 
+  EWcbvEval.eval (wfl:=wfl) p.1.(global_decls) p.2 t.
+
+Program Definition remove_params (p : eprogram_env) : eprogram :=
+  (ERemoveParams.strip_env p.1, ERemoveParams.strip p.1 p.2).
+
+Program Definition remove_params_optimization (fl : EWcbvEval.WcbvFlags) : 
+  Transform.t eprogram_env eprogram EAst.term EAst.term (eval_eprogram_env fl) (eval_eprogram fl) :=
+  {| name := "remove_parameters";
+    transform p pre := remove_params p;
+    pre p := 
+    let decls := p.1.(global_decls) in
+     [/\ wf_glob decls, ERemoveParams.isEtaExp_env decls, 
+      EEtaExpanded.isEtaExp decls p.2, closed_env decls & ELiftSubst.closedn 0 p.2];
+    post p := (closed_env p.1 /\ ELiftSubst.closedn 0 p.2);
+    obseq g g' v v' := v' = (ERemoveParams.strip g.1 v) |}.
+Next Obligation.
+  intros fl [Σ t] [wfe etae etat cle clt].
+  simpl.
+  cbn -[ERemoveParams.strip] in *.
+  split.
+  move: cle. unfold closed_env. unfold ERemoveParams.strip_env.
+  rewrite forallb_map. eapply forallb_impl. intros.
+  destruct x as [kn []]; cbn in * => //.
+  destruct E.cst_body => //. cbn -[ERemoveParams.strip] in H0 |- *.
+  now eapply ERemoveParams.closed_strip.
+  now eapply ERemoveParams.closed_strip.
+Qed.
+Next Obligation.
+  red. move=> [Σ t] /= v [wfe etae etat cle clt] ev.
+  eapply ERemoveParams.strip_eval in ev; eauto.
+Qed.
+
+Program Definition remove_params_fast_optimization (fl : EWcbvEval.WcbvFlags) :
+  Transform.t eprogram_env eprogram EAst.term EAst.term (eval_eprogram_env fl) (eval_eprogram fl) :=
+  {| name := "remove_parameters_fast";
     transform p _ := (ERemoveParams.Fast.strip_env p.1, ERemoveParams.Fast.strip p.1 [] p.2);
-    pre p := [/\ wf_glob p.1, ERemoveParams.isEtaExp_env p.1, ERemoveParams.isEtaExp p.1 p.2, closed_env p.1 & ELiftSubst.closedn 0 p.2];
+    pre p := 
+      let decls := p.1.(global_decls) in
+      [/\ wf_glob decls, ERemoveParams.isEtaExp_env decls, 
+       EEtaExpanded.isEtaExp decls p.2, closed_env decls & ELiftSubst.closedn 0 p.2];
     post p := (closed_env p.1 /\ ELiftSubst.closedn 0 p.2);
     obseq g g' v v' := v' = (ERemoveParams.strip g.1 v) |}.
 Next Obligation.
@@ -129,10 +191,9 @@ Next Obligation.
   cbn -[ERemoveParams.strip] in *.
   split.
   move: cle. unfold closed_env. unfold ERemoveParams.strip_env.
-  induction Σ at 1 3; cbn; auto.
-  move/andP => [] cla clg. rewrite (IHg clg) andb_true_r.
-  destruct a as [kn []]; cbn in * => //.
-  destruct E.cst_body => //. cbn -[ERemoveParams.strip] in cla |- *.
+  rewrite forallb_map. eapply forallb_impl. intros.
+  destruct x as [kn []]; cbn in * => //.
+  destruct E.cst_body => //. cbn -[ERemoveParams.strip] in H0 |- *.
   now eapply ERemoveParams.closed_strip.
   now eapply ERemoveParams.closed_strip.
 Qed.
@@ -142,38 +203,123 @@ Next Obligation.
   eapply ERemoveParams.strip_eval in ev; eauto.
 Qed.
 
+Definition pcuic_program := 
+  global_env_ext_map * term.
+
+Definition eval_program (p : Ast.Env.program) (v : Ast.term) :=
+  WcbvEval.eval p.1 p.2 v.  
+  
+Definition eval_pcuic_program (p : pcuic_program) (v : term) :=
+  PCUICWcbvEval.eval p.1.(trans_env_env) p.2 v.
+
+Definition template_to_pcuic_obseq (p : Ast.Env.program) (p' : pcuic_program) (v : Ast.term) (v' : term) :=
+  let Σ := Ast.Env.empty_ext p.1 in v' = trans (trans_global Σ) v.
+  
+Program Definition template_to_pcuic_transform {cf : checker_flags} : 
+  Transform.t Ast.Env.program pcuic_program Ast.term term 
+  eval_program eval_pcuic_program :=
+ {| name := "template to pcuic";
+    pre p :=  
+      let Σ := Ast.Env.empty_ext p.1 in
+      ∥ Typing.wf_ext Σ × ∑ T, Typing.typing (Ast.Env.empty_ext p.1) [] p.2 T ∥;
+    transform p hp := let Σ' := trans_global (Ast.Env.empty_ext p.1) in 
+      (Σ', trans Σ' p.2) ;
+    post p := ∥ wf_ext p.1 × ∑ T, typing p.1 [] p.2 T ∥;
+    obseq := template_to_pcuic_obseq |}.
+Next Obligation.
+  intros cf [Σ t] [[wfext ht]].
+  set (Σ' := trans_global _).
+  cbn. sq. split => //. eapply template_to_pcuic_env_ext. apply wfext.
+  destruct ht as [T HT]. exists (trans (trans_global_env Σ) T).
+  eapply (template_to_pcuic_typing (Σ := Ast.Env.empty_ext Σ) []). apply wfext.
+  apply HT.
+Qed.
+Next Obligation.
+  red. intros cf [Σ t] v [[]].
+  unfold eval_pcuic_program, eval_program.
+  cbn. intros ev.
+  unshelve eapply TemplateToPCUICWcbvEval.trans_wcbvEval in ev; eauto. apply w.
+  eexists; split; split; eauto. red. reflexivity.
+  eapply template_to_pcuic_env.
+  apply w. destruct s as [T HT]. apply TypingWf.typing_wf in HT. apply HT. auto.
+Qed.
+
+Program Definition build_global_env_map (g : global_env) : global_env_map := 
+  {| trans_env_env := g; 
+     trans_env_map := EnvMap.EnvMap.of_global_env g.(declarations) |}.
+Next Obligation.
+  intros g. eapply EnvMap.EnvMap.repr_global_env.
+Qed.
+
+Definition let_expansion_obseq (p : pcuic_program) (p' : pcuic_program) (v : term) (v' : term) :=
+  v' = PCUICExpandLets.trans v.
+
+Program Definition pcuic_expand_lets_transform {cf : checker_flags} : 
+  self_transform pcuic_program term eval_pcuic_program eval_pcuic_program :=
+ {| name := "let expansion in branches/constructors";
+    pre p :=
+      let Σ : global_env_ext := p.1 in
+      ∥ wf_ext Σ × ∑ T, typing Σ nil p.2 T ∥;
+    transform p hp := 
+      let Σ' := PCUICExpandLets.trans_global p.1 in 
+      ((build_global_env_map Σ', p.1.2), PCUICExpandLets.trans p.2) ;
+    post p := ∥ wf_ext (H:=PCUICExpandLetsCorrectness.cf' cf) p.1 × 
+      ∑ T, typing (H:=PCUICExpandLetsCorrectness.cf' cf) p.1 nil p.2 T ∥;
+    obseq := let_expansion_obseq |}.
+Next Obligation.
+  intros cf [Σ t] [[wfext ht]].
+  set (Σ' := PCUICExpandLets.trans_global _).
+  cbn. sq. unfold build_global_env_map. unfold global_env_ext_map_global_env_ext. simpl.
+  split. eapply PCUICExpandLetsCorrectness.trans_wf_ext in wfext. apply wfext.
+  destruct ht as [T HT]. exists (PCUICExpandLets.trans T).
+  eapply (PCUICExpandLetsCorrectness.pcuic_expand_lets Σ []) => //.
+  apply wfext. apply PCUICExpandLetsCorrectness.trans_wf_ext in wfext. apply wfext.
+Qed.
+Next Obligation.
+  red. intros cf [Σ t] v [[]].
+  unfold eval_pcuic_program.
+  cbn. intros ev.
+  unshelve eapply (PCUICExpandLetsCorrectness.trans_wcbveval (Σ:=Σ)) in ev; eauto.
+  eexists; split; split; eauto. red. reflexivity.
+  destruct s as [T HT]. now apply PCUICClosedTyp.subject_closed in HT.
+Qed.
+
 Obligation Tactic := program_simpl.
-Program Definition erase_template_program (p : Ast.Env.program) 
-  (wfΣ : ∥ Typing.wf_ext (Ast.Env.empty_ext p.1) ∥)
-  (wt : ∥ ∑ T, Typing.typing (Ast.Env.empty_ext p.1) [] p.2 T ∥)
-  : eprogram :=
-  let Σ0 := (trans_global (Ast.Env.empty_ext p.1)).1 in
-  let Σ := (PCUICExpandLets.trans_global_env Σ0) in
-  let wfΣ := map_squash (PCUICExpandLetsCorrectness.trans_wf_ext ∘
-    (template_to_pcuic_env_ext (Ast.Env.empty_ext p.1))) wfΣ in
-  let t := ErasureFunction.erase (build_wf_env_ext (empty_ext Σ) wfΣ) nil (PCUICExpandLets.trans (trans Σ0 p.2)) _ in
-  let Σ' := ErasureFunction.erase_global (term_global_deps t) Σ (sq_wf_ext wfΣ) in
-  (Σ', t).
+
+Definition build_wf_env_from_env {cf : checker_flags} (Σ : global_env_map) (wfΣ : ∥ wf Σ ∥) : wf_env := 
+  {| wf_env_env := Σ.(trans_env_env);
+     wf_env_map := Σ.(trans_env_map);
+     wf_env_map_repr := Σ.(trans_env_repr);
+     wf_env_wf := wfΣ;
+     wf_env_graph := (graph_of_wf wfΣ).π1;
+     wf_env_graph_wf := (graph_of_wf wfΣ).π2 |}.
+
+Program Definition erase_pcuic_program (p : pcuic_program) 
+  (wfΣ : ∥ wf_ext (H := config.extraction_checker_flags) p.1 ∥)
+  (wt : ∥ ∑ T, typing (H := config.extraction_checker_flags) p.1 [] p.2 T ∥) : eprogram_env :=
+  let wfe := build_wf_env_from_env p.1.1 (map_squash (wf_ext_wf _) wfΣ) in
+  let wfe' := make_wf_env_ext wfe p.1.2 wfΣ in
+  let t := ErasureFunction.erase wfe' nil p.2 _ in
+  let Σ' := ErasureFunction.erase_global (term_global_deps t) wfe in
+  (EEtaExpanded.GlobalContextMap.make Σ' _, t).
   
 Next Obligation.
   sq. destruct wt as [T Ht].
-  cbn.
-  set (Σ' := empty_ext _).
-  exists (PCUICExpandLets.trans (trans (trans_global_env p.1) T)).
-  change Σ' with (PCUICExpandLets.trans_global (trans_global (Ast.Env.empty_ext p.1))).
-  change (@nil (@BasicAst.context_decl term)) with (PCUICExpandLets.trans_local (trans_local (trans_global_env p.1) [])).
-  eapply (PCUICExpandLetsCorrectness.expand_lets_sound (cf := extraction_checker_flags)).
-  apply (template_to_pcuic_typing (Ast.Env.empty_ext p.1));simpl. apply wfΣ0.
-  apply Ht. Unshelve. now eapply template_to_pcuic_env.
-Defined.
+  cbn. now exists T.
+Qed.
+Next Obligation.
+  unfold erase_global.
+  eapply wf_glob_fresh.
+  eapply ERemoveParams.erase_global_decls_wf_glob.
+Qed.
 
-(** The full correctness lemma of erasure from Template programs do λ-box *)
+(* * The full correctness lemma of erasure from Template programs do λ-box
 
-Lemma erase_template_program_correctness {p : Ast.Env.program}
-  (Σ := Ast.Env.empty_ext p.1)
+Lemma erase_template_program_correctness {p : Ast.Env.program} univs
+  (Σ := (p.1, univs))
   {wfΣ : ∥ Typing.wf_ext Σ ∥}
-  {wt : ∥ ∑ T, Typing.typing (Ast.Env.empty_ext p.1) [] p.2 T ∥} {Σ' t'} :
-  erase_template_program p wfΣ wt = (Σ', t') ->
+  {wt : ∥ ∑ T, Typing.typing (p.1, univs) [] p.2 T ∥} {Σ' t'} :
+  erase_template_program p univs wfΣ wt = (Σ', t') ->
   forall v, WcbvEval.eval p.1 p.2 v ->
   exists v',
     PCUICExpandLets.trans_global (trans_global Σ) ;;; [] |- 
@@ -182,87 +328,106 @@ Lemma erase_template_program_correctness {p : Ast.Env.program}
 Proof.
   unfold erase_template_program.
   intros [= <- <-] v ev.
-  pose proof (erase_correct (PCUICExpandLets.trans_global (trans_global Σ))).
+  set (expΣ := (PCUICExpandLets.trans_global (trans_global Σ))).
+  set (wfexpΣ := build_wf_env _ _).
+  pose proof (erase_correct wfexpΣ).
+  set (wfexpΣ' := make_wf_env_ext _ _ _) in *.
   set wftΣ : ∥ wf_ext (PCUICExpandLets.trans_global (trans_global Σ)) ∥ :=
-    (map_squash (PCUICExpandLetsCorrectness.trans_wf_ext ∘ template_to_pcuic_env_ext (Ast.Env.empty_ext p.1)) wfΣ).
-  specialize (H wftΣ (PCUICExpandLets.trans (trans (trans_global Σ) p.2)) (PCUICExpandLets.trans (trans (trans_global Σ) v))).
+    wfexpΣ'.(wf_env_ext_wf).
+  specialize (H univs wftΣ (PCUICExpandLets.trans (trans (trans_global Σ) p.2)) (PCUICExpandLets.trans (trans (trans_global Σ) v))).
   set wtp : PCUICSafeLemmata.welltyped (PCUICExpandLets.trans_global (trans_global Σ)) [] 
     (PCUICExpandLets.trans (trans (trans_global Σ) p.2)) :=
-    (erase_template_program_obligation_1 p wfΣ wt).
-  set (t' := erase (build_wf_env_ext (empty_ext (PCUICExpandLets.trans_global (trans_global Σ)))
-    wftΣ) [] (PCUICExpandLets.trans (trans (trans_global Σ) p.2)) wtp).
+    (erase_template_program_obligation_1 p univs wfΣ wt).
+  set (t' := erase wfexpΣ' [] (PCUICExpandLets.trans (trans (trans_global_env p.1) p.2)) wtp) in *.
   set (deps := (term_global_deps _)).
-  change (empty_ext (PCUICExpandLets.trans_global_env (trans_global_env p.1))) with
-    (PCUICExpandLets.trans_global (trans_global Σ)) in *.
-  specialize (H (erase_global deps (PCUICExpandLets.trans_global (trans_global Σ)) (sq_wf_ext wftΣ))).
+  (* change (empty_ext (PCUICExpandLets.trans_global_env (trans_global_env p.1))) with *)
+    (* (PCUICExpandLets.trans_global (trans_global Σ)) in *. *)
+  specialize (H (erase_global deps wfexpΣ)).
   specialize (H _ deps wtp eq_refl).
   forward H. eapply Kernames.KernameSet.subset_spec. reflexivity.
   specialize (H eq_refl).
   destruct wt, wfΣ.
-  have wfmid : wf (trans_global (Ast.Env.empty_ext p.1)).1.
+  have wfmid : wf (trans_global (p.1, univs)).1.
   { now eapply template_to_pcuic_env. }
   forward H.
-  { eapply PCUICExpandLetsCorrectness.trans_wcbveval.
+  { unfold wfexpΣ. simpl.
+    unshelve eapply (PCUICExpandLetsCorrectness.trans_wcbveval (Σ := (trans_global_env p.1, univs))).
     { destruct s as [T HT].
-      eapply (PCUICClosedTyp.subject_closed (Γ := [])).
-      unshelve apply (template_to_pcuic_typing (Ast.Env.empty_ext p.1) [] _ T);simpl; eauto.
-      eapply w. }    
-    unshelve eapply trans_wcbvEval; eauto.
-    destruct s as [T HT].
+      eapply (PCUICClosedTyp.subject_closed (Γ := [])). 
+      apply (template_to_pcuic_typing (Σ := (p.1, univs)) [] _ T);simpl; eauto.
+      eapply w. Unshelve. now eapply template_to_pcuic_env. }
+    unshelve eapply trans_wcbvEval; eauto. apply w.
+    destruct s as [T HT]. eauto.
     clear -w HT. now eapply TypingWf.typing_wf in HT. }  
   destruct H as [v' [Hv He]].
   sq.
-  change (empty_ext (trans_global_env p.1)) with (trans_global Σ).
-  set (eΣ := erase_global _ _ _) in *. exists v'. split => //.
-Qed.
-
-Definition eval_program (p : Ast.Env.program) (v : Ast.term) :=
-  WcbvEval.eval p.1 p.2 v.
+  set (eΣ := erase_global _ _) in *. exists v'. split => //.
+Qed. *)
 
 Obligation Tactic := idtac.
 
-Program Definition erase_transform : Transform.t Ast.Env.program eprogram Ast.term EAst.term eval_program (eval_eprogram EWcbvEval.default_wcbv_flags) :=
- {| pre p :=  
-      let Σ := Ast.Env.empty_ext p.1 in
-      ∥ Typing.wf_ext Σ × ∑ T, Typing.typing (Ast.Env.empty_ext p.1) [] p.2 T ∥;
-    transform p hp := erase_template_program p (map_squash fst hp) (map_squash snd hp) ;
-    post p := (wf_glob p.1 /\ closed_env p.1 /\ ELiftSubst.closedn 0 p.2);
-    obseq g g' v v' :=
-      let Σ := Ast.Env.empty_ext g.1 in
-      PCUICExpandLets.trans_global (trans_global Σ) ;;; [] |- 
-      PCUICExpandLets.trans (trans (trans_global Σ) v) ⇝ℇ v' /\ 
-      ∥ EWcbvEval.eval (wfl:=EWcbvEval.default_wcbv_flags) g'.1 g'.2 v' ∥ |}.
+Program Definition erase_transform : Transform.t pcuic_program eprogram_env term EAst.term eval_pcuic_program (eval_eprogram_env EWcbvEval.default_wcbv_flags) :=
+ {| name := "erasure";
+    pre p :=  
+      ∥ wf_ext (H := config.extraction_checker_flags) p.1 × ∑ T, typing (H := config.extraction_checker_flags) p.1 [] p.2 T ∥;
+    transform p hp := erase_pcuic_program p (map_squash fst hp) (map_squash snd hp) ;
+    post p :=
+      let decls := p.1.(global_decls) in
+      [/\ wf_glob decls, closed_env decls & ELiftSubst.closedn 0 p.2];
+    obseq g g' v v' := let Σ := g.1 in Σ ;;; [] |- v ⇝ℇ v' |}.
 Next Obligation.
   intros [Σ t] [[wfext ht]].
-  destruct erase_template_program eqn:e.
-  unfold erase_template_program in e. simpl. injection e. intros <- <-. split.
-  eapply ERemoveParams.erase_global_wf_glob. split.
+  destruct erase_pcuic_program eqn:e.
+  unfold erase_pcuic_program in e. simpl. injection e. intros <- <-. split.
+  eapply ERemoveParams.erase_global_wf_glob.
   eapply erase_global_closed.
   eapply (erases_closed _ []). 2:eapply erases_erase.
   clear e. destruct ht as [T HT].
-  unshelve eapply (template_to_pcuic_typing _ []) in HT; eauto.
-  unshelve eapply PCUICClosedTyp.subject_closed in HT.
-  now eapply template_to_pcuic_env_ext. simpl in HT.
-  now eapply PCUICExpandLetsCorrectness.trans_closedn.
+  now eapply (@PCUICClosedTyp.subject_closed _ _) in HT.
 Qed.
 Next Obligation.
-  red. move=> [Σ t] v [[wf [T HT]]]. unfold eval_program.
+  red. move=> [Σ t] v [[wf [T HT]]]. unfold eval_pcuic_program, eval_eprogram.
   intros ev.
-  destruct erase_template_program eqn:e.
-  eapply (erase_template_program_correctness) in e; tea.
-  destruct e as [v' [he [hev]]]. exists v'; split; split => //.
+  destruct erase_pcuic_program eqn:e.
+  unfold erase_pcuic_program in e. simpl in e. injection e; intros <- <-.
+  simpl. clear e. cbn in *.
+  set (Σ' := build_wf_env_from_env _ _).
+  (* assert (wt : PCUICSafeLemmata.welltyped (cf:=config.extraction_checker_flags) Σ [] t). now exists T. *)
+  eapply (erase_correct Σ' Σ.2 _ _ _ _ _ (term_global_deps _)) in ev; try reflexivity.
+  2:eapply Kernames.KernameSet.subset_spec; reflexivity.
+  destruct ev as [v' [he [hev]]]. exists v'; split; split => //.
+  red. cbn.
+  eexact hev.
 Qed.
 
 Obligation Tactic := program_simpl.
+
+Local Notation " o ▷ o' " := (Transform.compose o o' _) (at level 50, left associativity).
+
 Program Definition erasure_pipeline := 
-  Transform.compose erase_transform 
-  (Transform.compose (remove_params_optimization _)
-    optimize_prop_discr_optimization _) _.
+  template_to_pcuic_transform ▷
+  pcuic_expand_lets_transform ▷
+  erase_transform ▷ 
+  remove_params_optimization _ ▷ 
+  optimize_prop_discr_optimization.
+
+Next Obligation.
+  sq. split => //. all:todo "etaexp".
+Qed.
+
+Definition erase_program := run erasure_pipeline.
+
+Program Definition erasure_pipeline_fast := 
+  template_to_pcuic_transform ▷
+  pcuic_expand_lets_transform ▷
+  erase_transform ▷ 
+  remove_params_fast_optimization _ ▷ 
+  optimize_prop_discr_optimization.
 Next Obligation.
   split => //. all:todo "etaexp".
 Qed.
 
-Definition erase_program := erasure_pipeline.(transform).
+Definition erase_program_fast := run erasure_pipeline_fast.
 
 Local Open Scope string_scope.
 
@@ -273,4 +438,9 @@ Local Open Scope string_scope.
 Program Definition erase_and_print_template_program {cf : checker_flags} (p : Ast.Env.program)
   : string :=
   let (Σ', t) := erase_program p (todo "wf_env and welltyped term") in
-  print_term Σ' [] true false t ^ nl ^ "in:" ^ nl ^ print_global_context Σ'.
+  time "Pretty printing" (fun _ => print_term Σ' [] true false t ^ nl ^ "in:" ^ nl ^ print_global_context Σ') tt.
+
+Program Definition erase_fast_and_print_template_program {cf : checker_flags} (p : Ast.Env.program)
+  : string :=
+  let (Σ', t) := erase_program_fast p (todo "wf_env and welltyped term") in
+  time "pretty-printing" (fun _ => print_term Σ' [] true false t ^ nl ^ "in:" ^ nl ^ print_global_context Σ') tt.
