erasure/theories/EExtends.v
@@ -1,0 +1,81 @@
+From MetaCoq.Template Require Import config utils Kernames.
+From MetaCoq.Erasure Require Import ETyping EAst Extract.
+
+Definition extends (Σ Σ' : global_declarations) := ∑ Σ'', Σ' = (Σ'' ++ Σ)%list.
+
+Definition fresh_global kn (Σ : global_declarations) :=
+  Forall (fun x => x.1 <> kn) Σ.
+
+Inductive wf_glob : global_declarations -> Type :=
+| wf_glob_nil : wf_glob []
+| wf_glob_cons kn d Σ : 
+  wf_glob Σ ->
+  fresh_global kn Σ ->
+  wf_glob ((kn, d) :: Σ).
+Derive Signature for wf_glob.
+
+Lemma lookup_env_Some_fresh {Σ c decl} :
+  lookup_env Σ c = Some decl -> ~ (fresh_global c Σ).
+Proof.
+  induction Σ; cbn. 1: congruence.
+  unfold BasicAst.eq_kername. destruct BasicAst.kername_eq_dec; subst.
+  - intros [= <-] H2. invs H2.
+    contradiction.
+  - intros H1 H2. apply IHΣ; tas.
+    now inv H2.
+Qed.
+
+Lemma extends_lookup {Σ Σ' c decl} :
+  wf_glob Σ' ->
+  extends Σ Σ' ->
+  lookup_env Σ c = Some decl ->
+  lookup_env Σ' c = Some decl.
+Proof.
+  intros wfΣ' [Σ'' ->]. simpl.
+  induction Σ'' in wfΣ', c, decl |- *.
+  - simpl. auto.
+  - specialize (IHΣ'' c decl). forward IHΣ''.
+    + now inv wfΣ'.
+    + intros HΣ. specialize (IHΣ'' HΣ).
+      inv wfΣ'. simpl in *. unfold BasicAst.eq_kername.
+      destruct BasicAst.kername_eq_dec; subst; auto.
+      apply lookup_env_Some_fresh in IHΣ''; contradiction.
+Qed.
+
+Lemma weakening_env_declared_constant :
+  forall Σ cst decl,
+    declared_constant Σ cst decl ->
+    forall Σ', wf_glob Σ' -> extends Σ Σ' -> declared_constant Σ' cst decl.
+Proof.
+  intros Σ cst decl H0 Σ' X2 H2.
+  eapply extends_lookup; eauto.
+Qed.
+
+Lemma weakening_env_declared_minductive :
+  forall Σ ind decl,
+    declared_minductive Σ ind decl ->
+    forall Σ', wf_glob Σ' -> extends Σ Σ' -> declared_minductive Σ' ind decl.
+Proof.
+  intros Σ cst decl H0 Σ' X2 H2.
+  eapply extends_lookup; eauto.
+Qed.
+
+Lemma weakening_env_declared_inductive:
+  forall Σ ind mdecl decl,
+    declared_inductive Σ mdecl ind decl ->
+    forall Σ', wf_glob Σ' -> extends Σ Σ' -> declared_inductive Σ' mdecl ind decl.
+Proof.
+  intros Σ cst decl H0 [Hmdecl Hidecl] Σ' X2 H2. split.
+  eapply weakening_env_declared_minductive; eauto.
+  eauto.
+Qed.
+
+Lemma weakening_env_declared_constructor :
+  forall Σ ind mdecl idecl decl,
+    declared_constructor Σ idecl ind mdecl decl ->
+    forall Σ', wf_glob Σ' -> extends Σ Σ' ->
+    declared_constructor Σ' idecl ind mdecl decl.
+Proof.
+  intros Σ cst mdecl idecl cdecl [Hidecl Hcdecl] Σ' X2 H2.
+  split; eauto. eapply weakening_env_declared_inductive; eauto.
+Qed.
