pcuic/theories/TemplateToPCUICWcbvEval.v
@@ -117,7 +117,7 @@ Proof.
 Qed.
 
 Ltac dest_lookup := 
-  destruct lookup_inductive as [[mdecl idecl]|].
+  destruct TransLookup.lookup_inductive as [[mdecl idecl]|].
   
 Lemma trans_csubst {cf} Σ a k b :
   Typing.wf Σ ->
@@ -471,7 +471,7 @@ Lemma isFixApp_trans Σ f : ~~ Ast.isApp f -> isFixApp (trans Σ f) -> WcbvEval.
 Proof.
   rewrite /isFixApp /WcbvEval.isFixApp.
   destruct f => //.
-  cbn. destruct lookup_inductive as [[]|]=> //.
+  cbn. destruct TransLookup.lookup_inductive as [[]|]=> //.
 Qed.
 
 Lemma eval_wf {cf} {Σ} {wfΣ : ST.wf Σ} {T U} :
@@ -538,18 +538,20 @@ Proof.
     eapply All2_All_right; tea; cbv beta; intuition auto.
 
   - wf_inv wf [mdecl' [idecl' []]].
-    eapply IHev.
+    eapply IHev2.
     econstructor; tea.
+    eapply IHev1 in w0.
     wf_inv w0 [hfix hargs].
     eapply WfAst.wf_mkApps => //.
     eapply wf_cunfold_cofix; tea. now depelim hfix.
 
   - wf_inv wf wf'.
-    wf_inv wf [hcofix hargs]. depelim hcofix.
-    eapply IHev.
+    eapply IHev2.
     econstructor; tea.
+    eapply IHev1 in wf.
+    wf_inv wf [hfix hargs].
     eapply WfAst.wf_mkApps => //.
-    eapply wf_cunfold_cofix; tea.
+    eapply wf_cunfold_cofix; tea. now depelim hfix.
     
   - wf_inv wf [[[hf ?]] ha].
     eapply WfAst.wf_mkApps; eauto.
@@ -575,8 +577,6 @@ Proof.
     cbn [trans].
     rewrite trans_mkApps in IHev3.
     cbn -[Σ']. 
-    (* cbn in cl; move: cl.
-    rewrite closedn_mkApps => /andP[] /= /andP[] clf clx cll. *)
     specialize (IHev1 wff). specialize (IHev2 wfx).
     cbn -[Σ'] in IHev1.
     pose proof (eval_wf wfx ev2).
@@ -608,6 +608,7 @@ Proof.
   - wf_inv wf [mdecl' [idecl' [decli ?]]].
     pose proof (declared_inductive_inj decli (proj1 H0)) as []. subst mdecl' idecl'.
     eapply forall_decls_declared_inductive in decli; tea.
+    rewrite trans_lookup_inductive.
     rewrite (declared_inductive_lookup _ decli).
     eapply All2_nth_error in a1; tea. 2:eapply H0.
     epose proof (forall_decls_declared_constructor _ _ _ _ _ _ _ H0) as decl'; tea.
@@ -704,29 +705,34 @@ Proof.
   
   - wf_inv wf [mdecl' [idecl' [decli ?]]].
     pose proof (forall_decls_declared_inductive _ _ _ _ _ _ decli) as decli';  tea.
+    rewrite trans_lookup_inductive.
     rewrite (declared_inductive_lookup _ decli').
-    eapply WfAst.wf_mkApps_napp in w0 as []; [|easy].
-    wf_inv w0 x.
-    rewrite trans_mkApps /=.  
-    eapply red_cofix_case.
-    eapply trans_cunfold_cofix; tea.
-    rewrite /= (declared_inductive_lookup _ decli') trans_mkApps in IHev.
-    apply IHev.
+    assert (w1 : WfAst.wf Σ (Ast.mkApps (Ast.tCoFix mfix idx) args))
+      by (eapply eval_wf; eauto).
+    eapply WfAst.wf_mkApps_napp in w1 as []; [|easy].
+    wf_inv w1 x. 
+    eapply eval_cofix_case.
+    eapply trans_cunfold_cofix; tea. 
+    rewrite trans_mkApps in IHev1.  eapply IHev1. eauto.
+    rewrite /= trans_lookup_inductive (declared_inductive_lookup _ decli') trans_mkApps in IHev2.
+    apply IHev2.
     econstructor; tea.
     eapply WfAst.wf_mkApps; tea.
     eapply wf_cunfold_cofix; tea.
 
-  - wf_inv wf [hfix hargs].
-    wf_inv wf [hfix ha].
+  - wf_inv wf [?].
+    forward IHev1. eauto.
+    assert (w1 : WfAst.wf Σ (Ast.mkApps (Ast.tCoFix mfix idx) args))
+      by (eapply eval_wf; eauto).
+    wf_inv w1 [hfix ha].
     depelim hfix.
-    forward IHev.
-    { constructor. eapply WfAst.wf_mkApps => //.
-      eapply wf_cunfold_cofix; tea. }
-    rewrite trans_mkApps /=.
-    eapply red_cofix_proj.
+    eapply eval_cofix_proj.
     eapply trans_cunfold_cofix; tea.
-    cbn in IHev. now rewrite trans_mkApps in IHev.
-
+    rewrite trans_mkApps in IHev1.  eapply IHev1.
+    cbn in IHev2. rewrite trans_mkApps in IHev2.  eapply IHev2.
+    econstructor.
+    eapply WfAst.wf_mkApps => //.
+    eapply wf_cunfold_cofix; tea.
   - wf_inv wf [[[] ?] ?].
     eapply All2_All_mix_left in X; tea.
     rewrite trans_mkApps.
@@ -757,7 +763,7 @@ Proof.
     auto. rewrite SisFixApp_mkApps.
     eapply isFixApp_trans in hp => //.
     rewrite H //.
-    cbn. destruct lookup_inductive as [[mdecl idecl]|]=> //.
+    cbn. destruct TransLookup.lookup_inductive as [[mdecl idecl]|]=> //.
     
   - eapply eval_atom.
     destruct t => //.
