test-suite/self_erasure.v
@@ -1,8 +1,7 @@
 From MetaCoq.Erasure Require Import Loader Erasure.
 From MetaCoq.SafeChecker Require Import PCUICSafeChecker.
-
-(* 32sec *)
-MetaCoq Erase @erase_and_print_template_program.
-
-(* 40sec *)
-Time MetaCoq Erase @typecheck_program.
+Set MetaCoq Timing.
+(* <1sec *)
+MetaCoq Fast Erase @erase_and_print_template_program.
+(* 2sec *)
+MetaCoq Fast Erase @typecheck_program.
